Add RTLC

x86/AsmregsC.v
@@ -6,6 +6,161 @@ Require Import MemoryC Integers AST.
 Require Export Asmregs.
 Require Import Locations.
 
+Set Implicit Arguments.
+
+
+
+Definition to_preg := preg_of.
+
+Definition to_mreg (pr: preg): option mreg :=
+  match pr with
+  | PC => None
+  | ST0 => Some FP0
+  | CR _ => None
+  | RA => None
+  | IR ir =>
+    match ir with
+    | RAX => Some AX
+    | RBX => Some BX
+    | RCX => Some CX
+    | RDX => Some DX
+    | RSI => Some SI
+    | RDI => Some DI
+    | RBP => Some BP
+    | RSP => None
+    | R8 => Some Machregs.R8
+    | R9 => Some Machregs.R9
+    | R10 => Some Machregs.R10
+    | R11 => Some Machregs.R11
+    | R12 => Some Machregs.R12
+    | R13 => Some Machregs.R13
+    | R14 => Some Machregs.R14
+    | R15 => Some Machregs.R15
+    end
+  | FR fr =>
+    match fr with
+    | XMM0 => Some X0
+    | XMM1 => Some X1
+    | XMM2 => Some X2
+    | XMM3 => Some X3
+    | XMM4 => Some X4
+    | XMM5 => Some X5
+    | XMM6 => Some X6
+    | XMM7 => Some X7
+    | XMM8 => Some X8
+    | XMM9 => Some X9
+    | XMM10 => Some X10
+    | XMM11 => Some X11
+    | XMM12 => Some X12
+    | XMM13 => Some X13
+    | XMM14 => Some X14
+    | XMM15 => Some X15
+    end
+  end
+.
+
+Lemma to_preg_to_mreg
+      mr0
+  :
+    mr0.(to_preg).(to_mreg) = Some mr0
+.
+Proof.
+  destruct mr0; ss.
+Qed.
+
+Lemma to_mreg_injective
+      pr0 pr1
+      (SOME: is_some (pr0.(to_mreg)))
+      (EQ: pr0.(to_mreg) = pr1.(to_mreg))
+  :
+    <<EQ: pr0 = pr1>>
+.
+Proof.
+  destruct pr0; ss; destruct pr1; ss; des_ifs.
+Qed.
+
+Lemma preg_of_injective
+      mr0 mr1
+      (EQ: preg_of mr0 = preg_of mr1)
+  :
+    <<EQ: mr0 = mr1>>
+.
+Proof. destruct mr0, mr1; ss. Qed.
+
+Lemma to_mreg_to_preg
+      pr0
+  :
+    o_map (pr0.(to_mreg)) (to_preg) = Some pr0 \/ pr0.(to_mreg) = None
+.
+Proof.
+  destruct pr0; ss; des_ifs; eauto.
+Qed.
+
+Corollary to_mreg_some_to_preg
+      pr0 mr0
+      (SOME: pr0.(to_mreg) = Some mr0)
+  :
+    <<EQ: mr0.(to_preg) = pr0>>
+.
+Proof.
+  eapply to_mreg_injective with (pr0 := mr0.(to_preg)) (pr1 := pr0).
+  { rewrite to_preg_to_mreg; ss. }
+  rewrite to_preg_to_mreg; ss.
+Qed.
+
+Print Conventions1.
+(* Note: callee_save registers all reside in mregs. So we can just put undef on preg\mreg. *)
+
+Definition is_callee_save (sg: signature) (pr: preg): bool :=
+  match pr.(to_mreg) with
+  | Some mr => Conventions1.is_callee_save mr
+  | None => false
+  end
+.
+(* Inductive is_callee_save (sg: signature) (pr: preg): Prop := *)
+(* | is_callee_save_some *)
+(*     mr *)
+(*     (MREG: pr.(to_mreg) = Some mr) *)
+(*     (CALLEESAVE: Conventions1.is_callee_save mr) *)
+(* . *)
+
+Inductive callee_saved (sg: signature) (rs0 rs1: regset): Prop :=
+| callee_saved_intro
+    (CALLEESAVE: forall
+        r
+        (CALLEESAVE: is_callee_save sg r = true)
+      ,
+        <<SAVE: (rs0 r) = (rs1 r)>>
+        (* <<SAVE: Val.lessdef (rs0 r) (rs1 r)>> *)
+    )
+(* In Compcert' sg is not needed (see is_callee_save). Is it true in real-world too? *)
+.
+
+Inductive fill_garbage (sg: signature) (rs0 rs1: regset): Prop :=
+| fill_garbage_intro
+    (CALLERSAVE: forall
+        r
+        (CALLERSAVE: is_callee_save sg r = false)
+      ,
+        <<GARBAGE: (rs1 r) = Vundef>>
+    )
+    (CALLEESAVE: forall
+        r
+        (CALLEESAVE: is_callee_save sg r = true)
+      ,
+        <<SAVE: (rs0 r) = (rs1 r)>>
+    (* <<SAVE: Val.lessdef (rs0 r) (rs1 r)>> *)
+    )
+.
+
+
+
+
+
+
+
+
+
 
 Module PLAYGROUND.
 (* Lemma extcall_arguments_perm_aux *)
@@ -160,8 +315,32 @@ Admitted.
 
 End PLAYGROUND.
 
-(* Reset size_arguments_loc_arguments. *)
+(* Reset PLAYGROUND. *)
 
+
+
+
+
+
+
+
+
+
+Inductive store_arguments (vs: list val) (m0: mem) (sg: signature):
+  regset -> mem -> Prop :=
+| store_arguments_intro
+    m1 sp
+    (ALLOC: Mem.alloc m0 Stacklayout.fe_ofs_arg (size_arguments sg) = (m1, sp))
+    (rs_arg: regset)
+    (RSPPTR: rs_arg RSP = Vptr sp Ptrofs.zero true)
+    m_arg
+    (STORE: extcall_arguments rs_arg m_arg sg vs /\ Mem.unchanged_on top2 m0 m_arg /\
+            m1.(Mem.nextblock) = m_arg.(Mem.nextblock) /\
+            (forall ofs (OUTSIDE: ~ 0 <= ofs < 4 * size_arguments sg), ~Mem.perm m_arg sp ofs Cur Nonempty) /\
+            Mem.range_perm m_arg sp 0 (4 * size_arguments sg) Cur Freeable)
+  :
+    store_arguments vs m0 sg rs_arg m_arg
+.
 
 Inductive load_arguments (rs_arg: regset) (m_arg: mem) (sg_init: signature)
           (vs_init: list val) (m_init: mem): Prop :=
@@ -173,126 +352,278 @@ Inductive load_arguments (rs_arg: regset) (m_arg: mem) (sg_init: signature)
     (DROP: Mem_set_perm m_arg sp 0 (4 * (size_arguments sg_init)) None = Some m_init)
 .
 
+Lemma load_arguments_dtm
+      rs_arg m_arg sg_init
+      vs_init0 vs_init1 m_init0 m_init1
+      (LOAD0: load_arguments rs_arg m_arg sg_init vs_init0 m_init0)
+      (LOAD1: load_arguments rs_arg m_arg sg_init vs_init1 m_init1)
+  :
+    vs_init0 = vs_init1 /\ m_init0 = m_init1
+.
+Proof.
+  inv LOAD0. inv LOAD1.
+  rewrite RSPPTR in *. clarify.
+  determ_tac extcall_arguments_determ.
+Qed.
+
+Definition dead_block (m: mem) (b: block): Prop := forall ofs, ~Mem.perm m b ofs Cur Nonempty.
+
+Lemma Mem_unchanged_on_trans_strong
+      P m0 m1 m2
+      (UNCH0: Mem.unchanged_on P m0 m1)
+      (UNCH1: Mem.unchanged_on (P /2\ (fun b _ => Mem.valid_block m0 b)) m1 m2)
+  :
+    <<UNCH2: Mem.unchanged_on P m0 m2>>
+.
+Proof.
+  inv UNCH0. inv UNCH1.
+  econs; i.
+  - xomega.
+  - etransitivity.
+    { eapply unchanged_on_perm; eauto. }
+    eapply unchanged_on_perm0; eauto.
+    { unfold Mem.valid_block in *. xomega. }
+  - erewrite <- unchanged_on_contents; eauto.
+    dup H0. apply Mem.perm_valid_block in H1. unfold Mem.valid_block in *.
+    erewrite <- unchanged_on_contents0; eauto.
+    eapply unchanged_on_perm; eauto.
+Qed.
+
+Local Opaque Z.mul.
+
+Theorem store_load_arguments_progress
+        vs0 m0 sg rs_arg m_arg
+        (STORE: store_arguments vs0 m0 sg rs_arg m_arg)
+  :
+    exists vs1 m1,
+      <<LOAD: load_arguments rs_arg m_arg sg vs1 m1>>
+.
+Proof.
+  inv STORE. des.
+  assert(exists m2, Mem_set_perm m_arg sp 0 (4 * size_arguments sg) None = Some m2).
+  { admit "it always suceeds". }
+  des.
+  esplits; eauto. econs; eauto.
+  - eapply Mem.range_perm_implies; eauto.
+    econs; eauto.
+Qed.
+
+Theorem store_load_arguments_spec
+        vs0 m0 sg rs_arg m_arg
+        (STORE: store_arguments vs0 m0 sg rs_arg m_arg)
+        vs1 m1
+        (LOAD: load_arguments rs_arg m_arg sg vs1 m1)
+  :
+    <<VAL: vs0 = vs1>> /\ <<MEM: Mem.unchanged_on top2 m0 m1
+                                 /\ dead_block m1 m0.(Mem.nextblock)
+                                 /\ Pos.succ m0.(Mem.nextblock) = m1.(Mem.nextblock)>>
+.
+Proof.
+  inv STORE. inv LOAD.
+  rewrite RSPPTR in *. clarify.
+  determ_tac extcall_arguments_determ; eauto.
+  exploit Mem_set_perm_none_spec; eauto. i; des.
+  assert(sp0 = (Mem.nextblock m0)).
+  { exploit Mem.alloc_result; eauto. }
+  clarify.
+  rename m1 into tt. rename m2 into m1. rename tt into m2.
+  esplits; eauto.
+  - eapply Mem_unchanged_on_trans_strong; eauto.
+    admit "Add to set_perm_none_spec. this should hold".
+  - hnf. ii.
+    destruct (classic (0 <= ofs < 4 * size_arguments sg)).
+    + eapply INSIDE; eauto.
+    + erewrite <- OUTSIDE in H; cycle 1.
+      { right. xomega. }
+      eapply STORE3; eauto.
+  - exploit Mem.nextblock_alloc; eauto. i; des. rewrite <- H.
+    rewrite STORE2.
+    admit "Add to set_perm_none_spec. this should hold".
+Qed.
 
 
-Definition to_preg := preg_of.
 
-Definition to_mreg (pr: preg): option mreg :=
-  match pr with
-  | PC => None
-  | ST0 => Some FP0
-  | CR _ => None
-  | RA => None
-  | IR ir =>
-    match ir with
-    | RAX => Some AX
-    | RBX => Some BX
-    | RCX => Some CX
-    | RDX => Some DX
-    | RSI => Some SI
-    | RDI => Some DI
-    | RBP => Some BP
-    | RSP => None
-    | R8 => Some Machregs.R8
-    | R9 => Some Machregs.R9
-    | R10 => Some Machregs.R10
-    | R11 => Some Machregs.R11
-    | R12 => Some Machregs.R12
-    | R13 => Some Machregs.R13
-    | R14 => Some Machregs.R14
-    | R15 => Some Machregs.R15
-    end
-  | FR fr =>
-    match fr with
-    | XMM0 => Some X0
-    | XMM1 => Some X1
-    | XMM2 => Some X2
-    | XMM3 => Some X3
-    | XMM4 => Some X4
-    | XMM5 => Some X5
-    | XMM6 => Some X6
-    | XMM7 => Some X7
-    | XMM8 => Some X8
-    | XMM9 => Some X9
-    | XMM10 => Some X10
-    | XMM11 => Some X11
-    | XMM12 => Some X12
-    | XMM13 => Some X13
-    | XMM14 => Some X14
-    | XMM15 => Some X15
-    end
+
+Inductive store_result (rs_init: regset) (v: val) (sg_init: signature): regset -> Prop :=
+| store_result_intro
+    rs_garbage rs_ret
+    (GARBAGE: fill_garbage sg_init rs_init rs_garbage)
+    (STORE: set_pair (loc_external_result sg_init) v rs_garbage = rs_ret)
+  :
+    store_result rs_init v sg_init rs_ret
+.
+
+Definition disjoint X (dec: forall x0 x1, {x0 = x1} + {x0 <> x1}) (rp: rpair X): bool :=
+  match rp with
+  | One _ => true
+  | Twolong x0 x1 => negb (dec x0 x1)
   end
 .
 
-Lemma to_preg_to_mreg
-      mr0
+Definition get_pair (rp: rpair preg) (rs: regset): val :=
+  match rp with
+  | One r0 => rs r0
+  | Twolong r0 r1 => Val.longofwords (rs r0) (rs r1)
+  end
+.
+
+Lemma longofwords_lessdef
+      retv
   :
-    mr0.(to_preg).(to_mreg) = Some mr0
+    <<LD: Val.lessdef (Val.longofwords (Val.hiword retv) (Val.loword retv)) retv>>
 .
 Proof.
-  destruct mr0; ss.
+  destruct retv; ss.
+  rewrite Int64.ofwords_recompose. econs; eauto.
 Qed.
 
-Lemma to_mreg_injective
-      pr0 pr1
-      (SOME: is_some (pr0.(to_mreg)))
-      (EQ: pr0.(to_mreg) = pr1.(to_mreg))
+Lemma longofwords_long
+      retv
+      (LONG: Val.has_type retv Tlong)
   :
-    <<EQ: pr0 = pr1>>
+    <<EQ: (Val.longofwords (Val.hiword retv) (Val.loword retv)) = retv>>
 .
 Proof.
-  destruct pr0; ss; destruct pr1; ss; des_ifs.
-Qed.
+  destruct retv; ss.
+  rewrite Int64.ofwords_recompose. econs; eauto.
+Abort.
 
-Lemma preg_of_injective
-      mr0 mr1
-      (EQ: preg_of mr0 = preg_of mr1)
-  :
-    <<EQ: mr0 = mr1>>
-.
-Proof. destruct mr0, mr1; ss. Qed.
 
-Lemma to_mreg_to_preg
-      pr0
+Lemma longofwords_long (* We need more strict type checking *)
+      retv
+      (LONG: exists i0, retv = Vlong i0)
   :
-    o_map (pr0.(to_mreg)) (to_preg) = Some pr0 \/ pr0.(to_mreg) = None
+    <<EQ: (Val.longofwords (Val.hiword retv) (Val.loword retv)) = retv>>
 .
 Proof.
-  destruct pr0; ss; des_ifs; eauto.
+  des. clarify. ss.
+  rewrite Int64.ofwords_recompose. econs; eauto.
 Qed.
 
-Corollary to_mreg_some_to_preg
-      pr0 mr0
-      (SOME: pr0.(to_mreg) = Some mr0)
+Lemma getpair_setpair
+      rp retv rs
+      (DISJ: disjoint preg_eq rp)
   :
-    <<EQ: mr0.(to_preg) = pr0>>
+    <<LD: Val.lessdef (get_pair rp (set_pair rp retv rs)) retv>>
 .
 Proof.
-  eapply to_mreg_injective with (pr0 := mr0.(to_preg)) (pr1 := pr0).
-  { rewrite to_preg_to_mreg; ss. }
-  rewrite to_preg_to_mreg; ss.
+  destruct rp; ss.
+  - unfold Pregmap.set. des_ifs.
+  - unfold Pregmap.set. simpl_bool. des_sumbool. des_ifs.
+    eapply longofwords_lessdef.
 Qed.
 
-Print Conventions1.
-(* Note: callee_save registers all reside in mregs. So we can just put undef on preg\mreg. *)
-
-Inductive is_callee_save (sg: signature) (pr: preg): Prop :=
-| is_callee_save_some
-    mr
-    (MREG: pr.(to_mreg) = Some mr)
-    (CALLEESAVE: Conventions1.is_callee_save mr)
-| is_callee_save_none
-    (MREG: pr.(to_mreg) = None)
+Inductive load_result (rs_arg: regset) (rs_ret: regset) (sg: signature): val -> Prop :=
+| load_result_intro
+    retv
+    (LOAD: get_pair (loc_external_result sg) rs_ret = retv)
+    (CALLEESAVE: callee_saved sg rs_arg rs_ret)
+  :
+    load_result rs_arg rs_ret sg retv
 .
 
-Inductive callee_saved (sg: signature) (rs0 rs1: regset): Prop :=
-| callee_saved_intro
-    (TODO: True)
-    (CALLEESAVE: forall
-        r
-        (CALLEESAVE: is_callee_save sg r)
-      ,
-        <<SAVE: Val.lessdef (rs0 r) (rs1 r)>>)
-(* In Compcert' sg is not needed (see is_callee_save). Is it true in real-world too? *)
+Lemma callee_saved_set
+      sg rs0 rs1
+      (SAVED: callee_saved sg rs0 rs1)
+      r0 v0
+      (NOTCALLEE: is_callee_save sg r0 = false)
+  :
+    <<SAVED: callee_saved sg rs0 (Pregmap.set r0 v0 rs1)>>
 .
+Proof.
+  inv SAVED.
+  econs; eauto.
+  ii. specialize (CALLEESAVE r CALLEESAVE0).
+  unfold Pregmap.set. des_ifs.
+Qed.
+
+Lemma callee_saved_set_pair
+      sg rs0 rs1
+      (SAVED: callee_saved sg rs0 rs1)
+      rp0 v0
+      (NOTCALLEE: forall_rpair (fun r => is_callee_save sg r = false) rp0)
+  :
+    <<SAVED: callee_saved sg rs0 (set_pair rp0 v0 rs1)>>
+.
+Proof.
+  unfold set_pair in *. des_ifs.
+  - eapply callee_saved_set; eauto.
+  - ss. des.
+    eapply callee_saved_set; eauto.
+    eapply callee_saved_set; eauto.
+Qed.
+
+Lemma loc_external_result_caller_save
+      sg
+  :
+    forall_rpair (fun pr => is_callee_save sg pr = false) (loc_external_result sg)
+.
+Proof.
+  hexploit (loc_result_caller_save sg); eauto. i.
+  unfold forall_rpair in *. unfold loc_external_result in *. unfold map_rpair in *. unfold is_callee_save in *.
+  des_ifs; ss; rewrite to_preg_to_mreg in *; clarify.
+Qed.
+
+Theorem store_load_result_progress
+        rs_arg retv0 sg rs_ret
+        (STORE: store_result rs_arg retv0 sg rs_ret)
+  :
+    exists retv1,
+      <<LOAD: load_result rs_arg rs_ret sg retv1>> /\ <<LD: Val.lessdef retv1 retv0>>
+.
+Proof.
+  inv STORE.
+  esplits.
+  - econs; eauto.
+    eapply callee_saved_set_pair; eauto.
+    { inv GARBAGE. econs; eauto. }
+    eapply (loc_external_result_caller_save sg); eauto.
+  - eapply getpair_setpair; eauto.
+    unfold loc_external_result. unfold loc_result, loc_result_64, loc_result_32. des_ifs.
+Qed.
+
+(* TODO: more specs? store_results always suceeds, load_result/store_result is dtm, etc. *)
+Theorem store_load_result_spec
+        rs_arg retv0 retv1 sg rs_ret
+        (STORE: store_result rs_arg retv0 sg rs_ret)
+        (LOAD: load_result rs_arg rs_ret sg retv1)
+  :
+    <<LD: Val.lessdef retv1 retv0>>
+.
+Proof.
+  inv STORE. inv LOAD.
+  esplits; eauto.
+  - eapply getpair_setpair; eauto.
+    unfold loc_external_result. unfold loc_result, loc_result_64, loc_result_32. des_ifs.
+Qed.
+
+Lemma fill_garbage_dtm
+      sg_init rs_init rs_garbage0 rs_garbage1
+      (GARBAGE0: fill_garbage sg_init rs_init rs_garbage0)
+      (GARBAGE1: fill_garbage sg_init rs_init rs_garbage1)
+  :
+    rs_garbage0 = rs_garbage1
+.
+Proof.
+  inv GARBAGE0. inv GARBAGE1.
+  apply Axioms.functional_extensionality.
+  i.
+  destruct (is_callee_save sg_init x) eqn:T.
+  - erewrite <- CALLEESAVE; eauto.
+    erewrite <- CALLEESAVE0; eauto.
+  - erewrite CALLERSAVE; eauto.
+    erewrite CALLERSAVE0; eauto.
+Qed.
+
+Lemma store_result_dtm
+      rs_init v_ret sg_init rs_ret0 rs_ret1
+      (STORE: store_result rs_init v_ret sg_init rs_ret0)
+      (STORE0: store_result rs_init v_ret sg_init rs_ret1)
+  :
+    <<EQ: rs_ret0 = rs_ret1>>
+.
+Proof.
+  inv STORE. inv STORE0.
+  determ_tac fill_garbage_dtm.
+Qed.
 
