backend/RTLC.v
@@ -1,0 +1,114 @@
+Require Import CoqlibC Maps.
+Require Import ASTC Integers Values Events Memory Globalenvs.
+Require Import Op Registers.
+Require Import sflib.
+Require Import SmallstepC.
+(** newly added **)
+Require Export RTL.
+Require Import ModSem.
+Require Import AsmregsC.
+Require Import Conventions.
+(* Require Import Locations. *)
+
+Set Implicit Arguments.
+
+
+
+
+
+Definition get_mem (st: state): mem :=
+  match st with
+  | State _ _ _ _ _ m0 => m0
+  | Callstate _ _ _ _ m0 => m0
+  | Returnstate _ _ m0 => m0
+  end
+.
+
+Section MODSEM.
+
+  Variable p: program.
+  Let ge := p.(Genv.globalenv).
+
+  Inductive at_external: state -> regset -> mem -> Prop :=
+  | at_external_intro
+      stack fptr_arg sg_arg vs_arg m0
+      m_arg sp
+      (ALLOC: Mem.alloc m_arg Stacklayout.fe_ofs_arg (size_arguments sg_arg) = (m_arg, sp))
+      rs_arg
+      (STORE: extcall_arguments rs_arg m_arg sg_arg vs_arg)
+      (EXTERNAL: Genv.find_funct ge fptr_arg = None)
+    :
+      at_external (Callstate stack fptr_arg sg_arg vs_arg m0)
+                  rs_arg m_arg
+  .
+
+  Inductive initial_frame (rs_arg: regset) (m_arg: mem)
+    : state -> Prop :=
+  | initial_frame_intro
+      fptr_arg fd
+      (FPTR: fptr_arg = rs_arg PC)
+      (FINDF: Genv.find_funct ge fptr_arg = Some (Internal fd))
+      vs_arg m_init
+      (LOAD: load_arguments rs_arg m_arg fd.(fn_sig) vs_arg m_init)
+    :
+      initial_frame rs_arg m_arg
+                    (Callstate [] fptr_arg fd.(fn_sig) vs_arg m_init)
+  .
+
+  Inductive final_frame (rs_init: regset): state -> regset -> Prop :=
+  | final_frame_intro
+      fd
+      (FINDF: Genv.find_funct ge (rs_init PC) = Some (Internal fd))
+      v_ret m_ret rs_ret
+      (STORE: store_result rs_init v_ret fd.(fn_sig) rs_ret)
+    :
+      final_frame rs_init (Returnstate [] v_ret m_ret) rs_ret
+  .
+
+  Inductive after_external: state -> regset -> regset -> mem -> state -> Prop :=
+  | after_external_intro
+      stack fptr_arg sg_arg vs_arg m_arg
+      rs_ret m_ret
+      v_ret rs_arg
+      (LOAD: load_result rs_arg rs_ret sg_arg v_ret)
+    :
+      after_external (Callstate stack fptr_arg sg_arg vs_arg m_arg)
+                     rs_arg
+                     rs_ret m_ret
+                     (Returnstate stack v_ret m_ret)
+  .
+
+  Program Definition modsem: ModSem.t :=
+    {|
+      ModSem.step := step;
+      ModSem.get_mem := get_mem;
+      ModSem.at_external := at_external;
+      ModSem.initial_frame := initial_frame;
+      ModSem.final_frame := final_frame;
+      ModSem.after_external := after_external;
+      ModSem.globalenv := ge; (* TODO: Change this properly *)
+      ModSem.skenv := (admit "TODO")
+    |}
+  .
+  Next Obligation. all_prop_inv; ss. Qed.
+  Next Obligation.
+    all_once_fast ltac:(fun H => try inv H).
+    rewrite FINDF in *. clarify.
+    determ_tac load_arguments_dtm.
+  Qed.
+  Next Obligation.
+    all_once_fast ltac:(fun H => try inv H); rewrite FINDF in *; clarify. determ_tac store_result_dtm.
+  Qed.
+  Next Obligation. all_prop_inv; ss. Qed.
+  Next Obligation.
+    ii; ss; des; all_once_fast ltac:(fun H => try inv H); rewrite EXTERNAL in *; clarify.
+  Qed.
+  Next Obligation.
+    ii; ss; des; all_once_fast ltac:(fun H => try inv H); rewrite EXTERNAL in *; clarify.
+  Qed.
+  Next Obligation.
+    ii; ss; des; all_once_fast ltac:(fun H => try inv H).
+  Qed.
+
+End MODSEM.
+
